move SelfClose earlier, and use it in Elims

src/SelfClose.v
@@ -16,7 +16,7 @@ Inductive expr :=
 | Deref : expr -> nat -> expr
 | Call : expr -> expr -> expr
 | MkConstr (tag : nat) (args : list expr)
-| Switch (cases : list expr)
+| Elim (loop : expr) (cases : list expr) (target : expr)
 | MkClose (f : function_name) (free : list expr)
 .
 
@@ -25,18 +25,6 @@ Definition env := list expr.
 Inductive is_value : expr -> Prop :=
 | IsValue : forall v, is_value (Value v).
 
-
-Definition unwrap e :=
-    match e with
-    | Value v => Some v
-    | _ => None
-    end.
-
-Definition unwrap_list := map_partial unwrap.
-
-(* Inductive value : expr -> Prop := *)
-(* | VConstr : forall tag args, Forall value args -> value (Constr tag args) *)
-(* | VClose : forall f free, Forall value free -> value (Close f free). *)
 
 (* Continuation-based step relation *)
 
@@ -68,23 +56,23 @@ Inductive sstep (E : env) : state -> state -> Prop :=
         nth_error free off = Some v ->
         sstep E (Run (Deref (Value (Close fname free)) off) a s k) (k v)
 
-| SConstrStep : forall fname vs e es a s k,
-        Forall is_value vs ->
-        ~ is_value e ->
-        sstep E (Run (MkConstr fname (vs ++ [e] ++ es)) a s k)
-                (Run e a s (fun v => Run (MkConstr fname (vs ++ [Value v] ++ es)) a s k))
-| SConstrDone : forall fname es vs a s k,
-        unwrap_list es = Some vs ->
-        sstep E (Run (MkConstr fname es) a s k) (k (Constr fname vs))
-
 | SCloseStep : forall fname vs e es a s k,
         Forall is_value vs ->
         ~ is_value e ->
         sstep E (Run (MkClose fname (vs ++ [e] ++ es)) a s k)
                 (Run e a s (fun v => Run (MkClose fname (vs ++ [Value v] ++ es)) a s k))
-| SCloseDone : forall fname es vs a s k,
-        unwrap_list es = Some vs ->
+| SCloseDone : forall fname vs a s k,
+        let es := map Value vs in
         sstep E (Run (MkClose fname es) a s k) (k (Close fname vs))
+
+| SConstrStep : forall fname vs e es a s k,
+        Forall is_value vs ->
+        ~ is_value e ->
+        sstep E (Run (MkConstr fname (vs ++ [e] ++ es)) a s k)
+                (Run e a s (fun v => Run (MkConstr fname (vs ++ [Value v] ++ es)) a s k))
+| SConstrDone : forall fname vs a s k,
+        let es := map Value vs in
+        sstep E (Run (MkConstr fname es) a s k) (k (Constr fname vs))
 
 | SCallL : forall e1 e2 a s k,
         ~ is_value e1 ->
@@ -100,10 +88,20 @@ Inductive sstep (E : env) : state -> state -> Prop :=
         sstep E (Run (Call (Value (Close fname free)) (Value arg)) a s k)
                 (Run body arg (Close fname free) k)
 
-| SSwitchinate : forall cases tag args s k case,
+| SElimStepLoop : forall loop cases target a s k,
+        ~ is_value loop ->
+        sstep E (Run (Elim loop cases target) a s k)
+                (Run loop a s (fun v => Run (Elim (Value v) cases target) a s k))
+| SElimStep : forall loop cases target a s k,
+        is_value loop ->
+        ~ is_value target ->
+        sstep E (Run (Elim loop cases target) a s k)
+                (Run target a s (fun v => Run (Elim loop cases (Value v)) a s k))
+| SEliminate : forall loop cases tag args a s k case,
+        is_value loop ->
         nth_error cases tag = Some case ->
-        sstep E (Run (Switch cases) (Constr tag args) s k)
-                (Run case (Constr tag args) s k)
+        sstep E (Run (Elim loop cases (Value (Constr tag args))) a s k)
+                (Run (Call (Call case loop) (Value (Constr tag args))) a s k)
 .
 
 
@@ -122,19 +120,6 @@ Require Import Metadata.
 
 Definition prog_type : Type := list expr * list metadata.
 Definition valtype := HigherValue.value.
-
-(*
-Inductive expr_value : expr -> valtype -> Prop :=
-| EvConstr : forall tag args1 args2,
-        Forall2 expr_value args1 args2 ->
-        expr_value (Constr tag args1)
-                   (HigherValue.Constr tag args2)
-| EvClose : forall tag free1 free2,
-        Forall2 expr_value free1 free2 ->
-        expr_value (Close tag free1)
-                   (HigherValue.Close tag free2)
-.
- *)
 
 Inductive is_callstate (prog : prog_type) : valtype -> valtype -> state -> Prop :=
 | IsCallstate : forall fname free av body,
@@ -170,13 +155,14 @@ Definition semantics (prog : prog_type) : Semantics.semantics :=
 Definition expr_rect_mut
         (P : expr -> Type)
         (Pl : list expr -> Type)
+    (HValue :   forall v, P (Value v))
     (HArg :     P Arg)
     (HSelf :    P Self)
-    (HValue :   forall v, P (Value v))
-    (HDeref :   forall e off, P e -> P (Deref e off))
+    (HDeref :   forall e n, P e -> P (Deref e n))
     (HCall :    forall f a, P f -> P a -> P (Call f a))
     (HConstr :  forall tag args, Pl args -> P (MkConstr tag args))
-    (HSwitch :  forall cases, Pl cases -> P (Switch cases))
+    (HElim :    forall loop cases target,
+        P loop -> Pl cases -> P target -> P (Elim loop cases target))
     (HClose :   forall f free, Pl free -> P (MkClose f free))
     (Hnil :     Pl [])
     (Hcons :    forall e es, P e -> Pl es -> Pl (e :: es))
@@ -191,23 +177,60 @@ Definition expr_rect_mut
         | Value v => HValue v
         | Arg => HArg
         | Self => HSelf
-        | Deref e off => HDeref e off (go e)
+        | Deref e n => HDeref e n (go e)
         | Call f a => HCall f a (go f) (go a)
         | MkConstr tag args => HConstr tag args (go_list args)
-        | Switch cases => HSwitch cases (go_list cases)
+        | Elim loop cases target =>
+                HElim loop cases target (go loop) (go_list cases) (go target)
         | MkClose f free => HClose f free (go_list free)
         end in go e.
 
+Definition expr_rect_mut'
+        (P : expr -> Type)
+        (Pl : list expr -> Type)
+    HValue HArg HSelf HDeref HCall HConstr HElim HClose Hnil Hcons
+    : (forall e, P e) * (forall es, Pl es) :=
+    let go := expr_rect_mut P Pl
+        HValue HArg HSelf HDeref HCall HConstr HElim HClose Hnil Hcons
+    in
+    let fix go_list es :=
+        match es as es_ return Pl es_ with
+        | [] => Hnil
+        | e :: es => Hcons e es (go e) (go_list es)
+        end in
+    (go, go_list).
+
 (* Useful wrapper for `expr_rect_mut with (Pl := Forall P)` *)
 Definition expr_ind' (P : expr -> Prop)
+    (HValue :   forall v, P (Value v))
     (HArg :     P Arg)
     (HSelf :    P Self)
-    (HValue :   forall v, P (Value v))
-    (HDeref :   forall e off, P e -> P (Deref e off))
+    (HDeref :   forall e n, P e -> P (Deref e n))
     (HCall :    forall f a, P f -> P a -> P (Call f a))
-    (HConstr :  forall tag args, Forall P args -> P (MkConstr tag args))
-    (HSwitch :  forall cases, Forall P cases -> P (Switch cases))
+    (HConstr :  forall c args, Forall P args -> P (MkConstr c args))
+    (HElim :    forall loop cases target,
+        P loop -> Forall P cases -> P target -> P (Elim loop cases target))
     (HClose :   forall f free, Forall P free -> P (MkClose f free))
     (e : expr) : P e :=
     ltac:(refine (@expr_rect_mut P (Forall P)
-        HArg HSelf HValue HDeref HCall HConstr HSwitch HClose _ _ e); eauto).
+        HValue HArg HSelf HDeref HCall HConstr HElim HClose _ _ e); eauto).
+
+
+Definition expr_eq_dec : forall (x y : expr), { x = y } + { x <> y }.
+induction x using expr_rect_mut with
+    (Pl := fun xs => forall ys, { xs = ys } + { xs <> ys });
+destruct ys + destruct y; try solve [right; discriminate | left; eauto].
+
+- (* Value *) destruct (value_eq_dec v v0); left + right; congruence.
+- (* Deref *) destruct (IHx y), (eq_nat_dec n n0); left + right; congruence.
+- (* Call *) destruct (IHx1 y1), (IHx2 y2); left + right; congruence.
+- (* MkConstr *) destruct (eq_nat_dec tag tag0), (IHx args0); left + right; congruence.
+- (* Elim *)
+  destruct (IHx1 y1); try solve [right; congruence].
+  destruct (IHx2 cases0); try solve [right; congruence].
+  destruct (IHx3 y2); try solve [right; congruence].
+  left. congruence.
+- (* MkClose *) destruct (eq_nat_dec f f0), (IHx free0); left + right; congruence.
+
+- (* cons *) destruct (IHx e), (IHx0 ys); left + right; congruence.
+Defined.
