src/MkCloseSelfOpt.v
@@ -1,0 +1,783 @@
+Require Import Common Monads.
+Require Import Metadata.
+Require String.
+Require Import ListLemmas.
+Require Import Forall3.
+Require Import StepLib.
+Require Import HigherValue.
+
+Require Import Psatz.
+
+Require Import SelfClose.
+
+Set Default Timeout 15.
+
+
+Fixpoint upvars_list' n acc :=
+    match n with
+    | 0 => acc
+    | S n => upvars_list' n (Deref Self n :: acc)
+    end.
+
+Definition upvars_list n := upvars_list' n [].
+
+
+Definition is_self_mk_close_dec (fname : nat) nfree f free :
+    { f = fname /\ free = upvars_list nfree } +
+    { f <> fname \/ free <> upvars_list nfree }.
+destruct (eq_nat_dec f fname); try solve [right; tauto].
+destruct (list_eq_dec expr_eq_dec free (upvars_list nfree)); try solve [right; tauto].
+left; tauto.
+Defined.
+
+
+Definition rewrite fname nfree : expr -> expr :=
+    let fix go e :=
+        let fix go_list es :=
+            match es with
+            | [] => []
+            | e :: es => go e :: go_list es
+            end in
+
+        match e with
+        | Value v => Value v
+        | Arg => Arg
+        | Self => Self
+        | Deref e n => Deref (go e) n
+        | Call f a => Call (go f) (go a)
+        | MkConstr tag args => MkConstr tag (go_list args)
+        | Elim loop cases target => Elim (go loop) (go_list cases) (go target)
+        | MkClose f free =>
+                if is_self_mk_close_dec fname nfree f free then
+                    Self
+                else
+                    MkClose f (go_list free)
+        end in go.
+
+Definition rewrite_list fname nfree :=
+    let go := rewrite fname nfree in
+    let fix go_list es :=
+        match es with
+        | [] => []
+        | e :: es => go e :: go_list es
+        end in go_list.
+
+Ltac refold_rewrite fname nfree :=
+    fold (rewrite_list fname nfree) in *.
+
+
+Fixpoint compile_cu' exprs nfrees n :=
+    match exprs, nfrees with
+    | [], [] => []
+    | e :: exprs, nfree :: nfrees =>
+            rewrite n nfree e :: compile_cu' exprs nfrees (S n)
+    | _, _ => []
+    end.
+
+Section compile_cu.
+Open Scope option_monad.
+
+Definition compile_cu (cu : list expr * list metadata) :
+        option (list expr * list metadata) :=
+    let '(exprs, metas) := cu in
+    match eq_nat_dec (length exprs) (length metas) with
+    | left Heq => Some Heq
+    | right _ => None
+    end >>= fun Hlen =>
+    let nfrees := map m_nfree metas in
+    Some (compile_cu' exprs nfrees 0, metas).
+
+End compile_cu.
+
+
+
+Inductive I_expr fname nfree : expr -> expr -> Prop :=
+| IValue : forall v, I_expr fname nfree (Value v) (Value v)
+| IArg : I_expr fname nfree Arg Arg
+| ISelf : I_expr fname nfree Self Self
+| IDeref : forall ae be n,
+        I_expr fname nfree ae be ->
+        I_expr fname nfree (Deref ae n) (Deref be n)
+| ICall : forall af aa bf ba,
+        I_expr fname nfree af bf ->
+        I_expr fname nfree aa ba ->
+        I_expr fname nfree (Call af aa) (Call bf ba)
+| IMkConstr : forall tag aargs bargs,
+        Forall2 (I_expr fname nfree) aargs bargs ->
+        I_expr fname nfree (MkConstr tag aargs) (MkConstr tag bargs)
+| IElim : forall aloop acases atarget bloop bcases btarget,
+        I_expr fname nfree aloop bloop ->
+        Forall2 (I_expr fname nfree) acases bcases ->
+        I_expr fname nfree atarget btarget ->
+        I_expr fname nfree (Elim aloop acases atarget) (Elim bloop bcases btarget)
+| IMkClose : forall fname' aargs bargs,
+        Forall2 (I_expr fname nfree) aargs bargs ->
+        I_expr fname nfree (MkClose fname' aargs) (MkClose fname' bargs)
+
+| IMkCloseSelf :
+        I_expr fname nfree (MkClose fname (upvars_list nfree)) Self
+.
+
+Inductive I (AE BE : env) : state -> state -> Prop :=
+| IRun : forall a ae ak be bk fname free,
+        I_expr fname (length free) ae be ->
+        (forall v, I AE BE (ak v) (bk v)) ->
+        I AE BE (Run ae a (Close fname free) ak) (Run be a (Close fname free) bk)
+
+| IInMkClose1 : forall i es a fname free ak bk,
+        i <= length free ->
+        sliding i (map Value free) (upvars_list (length free)) es ->
+        (forall v, I AE BE (ak v) (bk v)) ->
+        I AE BE
+            (Run (MkClose fname es) a (Close fname free) ak)
+            (Run Self a (Close fname free) bk)
+
+| IInMkClose2 : forall i es1 es2 a fname free ak bk,
+        sliding (length es1) (map Value free) (upvars_list (length free))
+            (es1 ++ [Deref Self i] ++ es2) ->
+        (forall v, I AE BE (ak v) (bk v)) ->
+        I AE BE
+            (Run (Deref Self i) a (Close fname free) (fun v =>
+                Run (MkClose fname (es1 ++ [Value v] ++ es2)) a (Close fname free) ak))
+            (Run Self a (Close fname free) bk)
+
+| IInMkClose3 : forall i es1 es2 a fname free ak bk,
+        sliding (length es1) (map Value free) (upvars_list (length free))
+            (es1 ++ [Deref Self i] ++ es2) ->
+        (forall v, I AE BE (ak v) (bk v)) ->
+        I AE BE
+            (Run Self a (Close fname free) (fun v =>
+                Run (Deref (Value v) i) a (Close fname free) (fun v =>
+                    Run (MkClose fname (es1 ++ [Value v] ++ es2)) a (Close fname free) ak)))
+            (Run Self a (Close fname free) bk)
+
+| IInMkClose4 : forall i es1 es2 a fname free ak bk,
+        sliding (length es1) (map Value free) (upvars_list (length free))
+            (es1 ++ [Deref Self i] ++ es2) ->
+        (forall v, I AE BE (ak v) (bk v)) ->
+        I AE BE
+            (Run (Deref (Value (Close fname free)) i) a (Close fname free) (fun v =>
+                Run (MkClose fname (es1 ++ [Value v] ++ es2)) a (Close fname free) ak))
+            (Run Self a (Close fname free) bk)
+
+| IStop : forall v,
+        I AE BE (Stop v) (Stop v).
+
+
+
+Ltac i_ctor := intros; econstructor; simpl; eauto.
+Ltac i_lem H := intros; eapply H; simpl; eauto.
+
+
+Lemma rewrite_I_expr : forall fname nfree a b,
+    rewrite fname nfree a = b ->
+    I_expr fname nfree a b.
+intros ? ?.
+mut_induction a using expr_rect_mut' with
+    (Pl := fun as_ => forall bs,
+        rewrite_list fname nfree as_ = bs ->
+        Forall2 (I_expr fname nfree) as_ bs);
+[ intros0 Hrw; simpl in Hrw; refold_rewrite fname nfree;
+  try solve [subst b + subst bs; i_ctor].. | ].
+
+- (* MkClose *)
+  break_match.
+  + subst b.  break_and. subst.  i_lem IMkCloseSelf.
+  + subst b. i_ctor.
+
+- finish_mut_induction rewrite_I_expr using list.
+Qed.
+
+
+
+Lemma I_expr_value : forall fname nfree a b,
+    I_expr fname nfree a b ->
+    is_value a ->
+    is_value b.
+intros0 II Aval. invc Aval. invc II. constructor.
+Qed.
+Hint Resolve I_expr_value.
+
+Lemma I_expr_value' : forall fname nfree a b,
+    I_expr fname nfree a b ->
+    is_value b ->
+    is_value a.
+intros0 II Bval. invc Bval. invc II. constructor.
+Qed.
+Hint Resolve I_expr_value'.
+
+Lemma I_expr_not_value : forall fname nfree a b,
+    I_expr fname nfree a b ->
+    ~ is_value a ->
+    ~ is_value b.
+intros0 II Aval. contradict Aval. eauto using I_expr_value'.
+Qed.
+Hint Resolve I_expr_not_value.
+
+Lemma I_expr_not_value' : forall fname nfree a b,
+    I_expr fname nfree a b ->
+    ~ is_value b ->
+    ~ is_value a.
+intros0 II Bval. contradict Bval. eauto using I_expr_value.
+Qed.
+Hint Resolve I_expr_not_value'.
+
+Lemma I_expr_map_value : forall fname nfree vs bes,
+    Forall2 (I_expr fname nfree) (map Value vs) bes ->
+    bes = map Value vs.
+induction vs; intros0 II; invc II.
+- reflexivity.
+- simpl. f_equal.
+  + on >I_expr, invc. reflexivity.
+  + apply IHvs. eauto.
+Qed.
+
+
+
+Lemma upvars_list'_length : forall n acc,
+    length (upvars_list' n acc) = n + length acc.
+induction n; intros; simpl.
+- reflexivity.
+- rewrite IHn. simpl. omega.
+Qed.
+
+Lemma upvars_list_length : forall n,
+    length (upvars_list n) = n.
+intros. unfold upvars_list. rewrite upvars_list'_length. simpl. omega.
+Qed.
+
+Lemma upvars_list'_prefix : forall n acc,
+    exists prefix,
+        length prefix = n /\
+        upvars_list' n acc = prefix ++ acc.
+induction n; intros; simpl.
+- exists []. split; eauto.
+- specialize (IHn (Deref Self n :: acc)). break_exists. break_and.
+  exists (x ++ [Deref Self n]). split.
+  + rewrite app_length. simpl. omega.
+  + rewrite <- app_assoc. simpl. auto.
+Qed.
+
+Lemma upvars_list'_nth_error : forall n acc i,
+    i < n ->
+    nth_error (upvars_list' n acc) i = Some (Deref Self i).
+induction n; intros0 Hlt; simpl in *.
+- omega.
+- destruct (eq_nat_dec i n).
+  + subst.
+    fwd eapply upvars_list'_prefix with (n := n) (acc := Deref Self n :: acc).
+      break_exists. break_and.  on _, fun H => rewrite H.
+    change (?a ++ ?b :: ?c) with (a ++ [b] ++ c).
+    rewrite app_assoc. 
+    rewrite nth_error_app1 by (rewrite app_length; simpl; omega).
+    rewrite nth_error_app2 by omega.
+    replace (n - length x) with 0 by omega.
+    reflexivity.
+  + rewrite IHn; eauto. omega.
+Qed.
+
+Lemma upvars_list_nth_error : forall n i,
+    i < n ->
+    nth_error (upvars_list n) i = Some (Deref Self i).
+intros. unfold upvars_list. rewrite upvars_list'_nth_error; eauto.
+Qed.
+
+
+Lemma upvars_list_hd : forall n e es,
+    upvars_list n = e :: es ->
+    e = Deref Self 0.
+intros.
+assert (nth_error (upvars_list n) 0 = Some e).
+  { on _, fun H => rewrite H. reflexivity. }
+on _, rewrite_fwd upvars_list_nth_error; cycle 1.
+  { destruct n; try discriminate. lia. }
+congruence.
+Qed.
+
+Lemma upvars'_list_not_value : forall n acc,
+    Forall (fun e => ~ is_value e) acc ->
+    Forall (fun e => ~ is_value e) (upvars_list' n acc).
+induction n; intros0 Hfa; simpl in *.
+  { auto. }
+eapply IHn. i_ctor. inversion 1.
+Qed.
+
+Lemma upvars_list_not_value : forall n,
+    Forall (fun e => ~ is_value e) (upvars_list n).
+intros. unfold upvars_list. i_lem upvars'_list_not_value.
+Qed.
+
+Lemma map_inj : forall {A B} (f : A -> B) xs ys,
+    (forall x y, f x = f y -> x = y) ->
+    map f xs = map f ys -> xs = ys.
+induction xs; destruct ys; intros0 Hinj Hmap; simpl in *; try discriminate.
+- reflexivity.
+- invc Hmap. erewrite Hinj with (x := a); eauto.
+  erewrite IHxs; eauto.
+Qed.
+
+
+
+Definition metric (a : state) := 0.
+
+Theorem I_sim : forall AE BE NFREES a a' b,
+    Forall3 (fun a fname_b nfree => let '(fname, b) := fname_b in
+        I_expr fname nfree a b) AE (numbered BE) NFREES ->
+    I AE BE a b ->
+    sstep AE a a' ->
+    exists b',
+        (sstep BE b b' \/ (b' = b /\ metric a' < metric a)) /\
+        I AE BE a' b'.
+destruct a as [ae al ak | v];
+intros0 Henv II Astep; inv Astep.
+all: invc II.
+all: try on (I_expr _ _ _ be), invc.
+
+- (* SArg *)
+  eexists. split. left. i_lem SArg.
+  auto.
+
+- (* SSelf *)
+  eexists. split. left. i_lem SSelf.
+  auto.
+
+- (* SSelf - IInMkClose3 *)
+  eexists. split. right. split. reflexivity.
+    { (* metric *) admit. }
+  i_lem IInMkClose4.
+
+- (* SDerefStep *)
+  eexists. split. left. i_lem SDerefStep.
+  i_ctor. intros. eapply IRun with (fname := fname) (free := free); eauto. 
+  i_ctor. i_ctor.
+
+- (* SDerefStep - IInMkClose2 *)
+  eexists. split. right. split. reflexivity.
+    { (* metric *) admit. }
+  i_lem IInMkClose3.
+
+- (* SDerefStep - IInMkClose4 *)
+  on (~ is_value (Value _)), contradict. i_ctor.
+
+- (* SDerefinateConstr *)
+  on (I_expr _ _ (Value _) _), invc.
+  eexists. split. left. i_lem SDerefinateConstr.
+  eauto.
+
+- (* SDerefinateClose *)
+  on (I_expr _ _ (Value _) _), invc.
+  eexists. split. left. i_lem SDerefinateClose.
+  eauto.
+
+- (* SDerefinateClose - IInMkClose4 *)
+  assert (length es1 < length free).
+    { on _, eapply_lem sliding_length; cycle 1.
+        { rewrite map_length, upvars_list_length. reflexivity. }
+      do 2 on _, rewrite_fwd app_length. on _, rewrite_fwd map_length. simpl in *.
+      lia. }
+
+  eexists. split. right. split. reflexivity.
+    { (* metric *) admit. }
+  i_lem IInMkClose1.  i_lem sliding_next'.  eapply map_nth_error.
+  assert (length es1 = off).
+    { fwd eapply sliding_nth_error_ge with (i := length es1) (j := length es1); eauto.
+      on _, rewrite_fwd nth_error_app2; eauto.  replace (_ - _) with 0 in * by lia.
+      on _, rewrite_fwd upvars_list_nth_error; eauto.
+      simpl in *. congruence. }
+  congruence.
+
+- (* SCloseStep *)
+  on _, invc_using Forall2_3part_inv.
+  eexists. split. left. i_lem SCloseStep.
+  + list_magic_on (vs, (ys1, tt)).
+  + i_ctor. intros. eapply IRun with (fname := fname0) (free := free); eauto.
+    i_ctor. i_lem Forall2_app. i_ctor. i_ctor.
+
+- (* SCloseStep - IMkCloseSelf *)
+  destruct vs; cycle 1.
+    { exfalso. simpl in *. on _, eapply_lem upvars_list_hd. subst e0.
+      on >Forall, invc. on >is_value, invc. }
+
+  simpl in *. fwd i_lem upvars_list_hd. subst e.
+
+  eexists. split. right. split. reflexivity.
+    { (* metric *) admit. }
+  eapply IInMkClose2 with (i := 0) (es1 := []); eauto.
+  simpl. on _, fun H => rewrite <- H. i_lem sliding_zero.
+
+- (* SCloseStep - IInMkClose1 *)
+  assert (Forall is_value (map Value free)).
+    { rewrite <- Forall_map. rewrite Forall_forall. intros. constructor. }
+  fwd eapply upvars_list_not_value with (n := length free).
+
+  assert (length vs < length free).
+    { fwd eapply sliding_length. 2: eauto.
+        { rewrite map_length, upvars_list_length. reflexivity. }
+      rewrite app_length, map_length in *. simpl in *. lia. }
+
+  fwd eapply sliding_predicate_nth; [ simpl | .. ]; eauto.
+  fwd eapply sliding_predicate_i; [ simpl | .. ]; eauto.
+  rewrite upvars_list_nth_error in * by lia. inject_some.
+
+  eexists. split. right. split. reflexivity.
+    { (* metric *) admit. }
+  i_lem IInMkClose2.
+
+- (* SCloseDone *)
+  fwd i_lem I_expr_map_value. subst.
+  eexists. split. left. i_lem SCloseDone.
+  eauto.
+
+- (* SCloseDone - IMkCloseSelf *)
+  fwd eapply upvars_list_not_value with (n := length free).
+  on (upvars_list _ = map Value vs), fun H => rewrite H in *.
+  destruct vs; cycle 1; simpl in *.
+    { exfalso. on >Forall, invc.
+      on (~ is_value (Value _)), contradict. constructor. }
+
+  assert (length free = 0).
+    { rewrite <- upvars_list_length at 1. on _, fun H => rewrite H.  reflexivity. }
+  destruct free; try discriminate.
+
+  eexists. split. left. i_lem SSelf.
+  eauto.
+
+- (* SCloseDone - IInMkClose1 *)
+  fwd eapply sliding_predicate_all with (P := is_value); eauto.
+    { rewrite <- Forall_map, Forall_forall. i_ctor. }
+    { eapply upvars_list_not_value. }
+    { unfold es. rewrite <- Forall_map, Forall_forall. i_ctor. }
+
+  assert (i = length (map Value free)).
+    { rewrite map_length. rewrite upvars_list_length in *. lia. }
+  subst i.
+
+  fwd eapply sliding_all_eq; eauto.
+  subst es.  fwd eapply map_inj. 2: eassumption. { intros. congruence. }
+  subst vs.
+
+  eexists. split. left. i_lem SSelf.
+  eauto.
+
+- (* SConstrStep *)
+  on _, invc_using Forall2_3part_inv.
+  eexists. split. left. i_lem SConstrStep.
+  + list_magic_on (vs, (ys1, tt)).
+  + i_ctor. intros. eapply IRun with (fname := fname0) (free := free); eauto.
+    i_ctor. i_lem Forall2_app. i_ctor. i_ctor.
+
+- (* SConstrDone *)
+  fwd i_lem I_expr_map_value. subst.
+  eexists. split. left. i_lem SConstrDone.
+  eauto.
+
+- (* SCallL *)
+  eexists. split. left. i_lem SCallL.
+  i_ctor. i_ctor. i_ctor. i_ctor.
+
+- (* SCallR *)
+  eexists. split. left. i_lem SCallR.
+  i_ctor. i_ctor. i_ctor. i_ctor.
+
+- (* SMakeCall *)
+  on (I_expr _ _ _ bf), invc.
+  on (I_expr _ _ _ ba), invc.
+  fwd eapply Forall3_nth_error_ex1 as HH; eauto.
+    destruct HH as ([fname' bbody] & nfree & ? & ? & ?).
+  fwd i_lem numbered_nth_error_fst.
+  fwd i_lem numbered_nth_error_snd.
+  simpl in *. subst fname'.
+
+  assert (length free = nfree).
+    { (* nfree_ok *) admit. }
+
+  eexists. split. left. i_lem SMakeCall.
+  i_ctor. congruence.
+
+- (* SElimStepLoop *)
+  eexists. split. left. i_lem SElimStepLoop.
+  i_ctor. i_ctor. i_ctor. i_ctor.
+
+- (* SElimStep *)
+  eexists. split. left. i_lem SElimStep.
+  i_ctor. i_ctor. i_ctor. i_ctor.
+
+- (* SEliminate *)
+  on (I_expr _ _ _ btarget), invc.
+  fwd i_lem Forall2_nth_error_ex as HH.  destruct HH as (bcase & ? & ?).
+
+  eexists. split. left. i_lem SEliminate.
+  i_ctor. i_ctor. i_ctor. i_ctor.
+
+Admitted.
+
+
+(* TODO
+
+
+Inductive I' AE BE NFREES : A.state -> B.state -> Prop :=
+| I'_intro : forall a b,
+        I AE BE a b ->
+        A.nfree_ok_state NFREES a ->
+        I' AE BE NFREES a b.
+
+Definition env_ok AE BE NFREES :=
+    Forall3 (fun a b nfree => I_expr BE nfree [] a b) AE (firstn (length AE) BE) NFREES /\
+    Forall (A.nfree_ok NFREES) AE.
+
+Theorem I'_sim : forall AE BE NFREES a a' b,
+    env_ok AE BE NFREES ->
+    I' AE BE NFREES a b ->
+    A.sstep AE a a' ->
+    exists b',
+        B.splus BE b b' /\
+        I' AE BE NFREES a' b'.
+intros0 Henv II Astep.
+unfold env_ok in *. break_and.
+set (BE0 := firstn (length AE) BE).
+set (BE1 := skipn (length AE) BE).
+replace (firstn (length AE) BE) with BE0 in * by reflexivity.
+replace BE with (BE0 ++ BE1) in * by eapply firstn_skipn.
+
+intros. on >I', invc.
+fwd eapply I_sim; eauto. break_exists; break_and.
+eexists; split; eauto. constructor; eauto.
+eapply A.step_nfree_ok; try eassumption.
+Qed.
+
+
+
+Lemma compile_cu'_state_monotonic : forall base exprs metas s exprs' s',
+    compile_cu' base exprs metas s = Some (exprs', s') ->
+    exists s1, s' = s ++ s1.
+induction exprs; destruct metas; intros; simpl in *;
+  try discriminate; break_bind_state_option.
+  { exists []. eauto using app_nil_r. }
+
+on _, eapply_lem compile_state_monotonic.
+on _, eapply_lem IHexprs.
+break_exists. subst.
+eexists. rewrite app_assoc. reflexivity.
+Qed.
+
+Lemma compile_cu'_I_expr : forall BE0 aes ms s bes s',
+    length aes = length ms ->
+    compile_cu' (length BE0) aes ms s = Some (bes, s') ->
+    Forall3 (fun ae be nfree => I_expr (BE0 ++ map fst s') nfree [] ae be)
+        aes bes (map m_nfree ms).
+induction aes; destruct ms; intros0 Hlen Hcomp; simpl in *;
+  try discriminate; break_bind_state_option.
+  { constructor. }
+
+rename a into ae, x into be, x0 into bes.
+on _, eapply_lem compile_I_expr.
+fwd eapply compile_cu'_state_monotonic as HH; eauto.  destruct HH as [ssuffix ?H].
+on _, eapply_lem IHaes; [ | lia].
+i_ctor.
+subst s'. rewrite map_app, app_assoc. i_lem I_expr_weaken.
+Qed.
+
+Lemma compile_cu'_length : forall base exprs metas s exprs' s',
+    length exprs = length metas ->
+    compile_cu' base exprs metas s = Some (exprs', s') ->
+    length exprs' = length exprs.
+induction exprs; destruct metas; intros; simpl in *;
+  try discriminate; break_bind_state_option.
+- reflexivity.
+- simpl. f_equal. on _, eapply_lem IHexprs; eauto.
+Qed.
+
+Lemma process_recorded_fst : forall recs n,
+    fst (process_recorded recs n) = map fst recs.
+induction recs; intros.
+- reflexivity.
+- simpl. do 2 break_match; try discriminate.
+  simpl. f_equal. erewrite <- IHrecs. on _, fun H => rewrite H. reflexivity.
+Qed.
+
+Theorem compile_cu_env_ok : forall A Ameta B Bmeta,
+    compile_cu (A, Ameta) = Some (B, Bmeta) ->
+    env_ok A B (map m_nfree Ameta).
+intros. simpl in *. repeat (break_bind_option || break_match; try discriminate).
+inject_some.
+rename l into B0, l0 into B1_B1meta, l1 into B1, l2 into B1meta.
+rename Heqo1 into Hcomp.
+
+fwd eapply compile_cu'_length as Hlen; eauto.
+  rewrite <- Hlen in Hcomp.
+
+fwd eapply compile_cu'_I_expr; [ | eauto | ]; [ congruence | ].
+
+replace (map fst B1_B1meta) with B1 in *; cycle 1.
+  { erewrite <- process_recorded_fst. on _, fun H => rewrite H. reflexivity. }
+
+unfold env_ok.
+rewrite firstn_app by lia. rewrite firstn_all by lia.
+split; eauto.
+Qed.
+
+
+Lemma process_recorded_private : forall recs n exprs metas,
+    process_recorded recs n = (exprs, metas) ->
+    Forall (fun m => m_access m = Private) metas.
+induction recs; intros0 Hproc; simpl in *.
+- inject_pair. constructor.
+- do 2 break_match; try discriminate. inject_pair.
+  econstructor; eauto.
+Qed.
+
+Lemma compile_cu_meta_split : forall A Ameta B Bmeta,
+    compile_cu (A, Ameta) = Some (B, Bmeta) ->
+    exists Bnew_meta,
+        Forall (fun m => m_access m = Private) Bnew_meta /\
+        Bmeta = Ameta ++ Bnew_meta.
+intros0 Hcomp. unfold compile_cu in Hcomp. break_bind_option.
+do 4 (break_match; try discriminate).  do 3 inject_some.
+rename l into B0, l0 into B1_B1meta, l1 into B1, l2 into B1meta.
+exists B1meta. split; eauto using process_recorded_private.
+Qed.
+
+Lemma compile_cu_a_length : forall A Ameta B Bmeta,
+    compile_cu (A, Ameta) = Some (B, Bmeta) ->
+    length A = length Ameta.
+intros0 Hcomp. unfold compile_cu in Hcomp. break_bind_option.
+assumption.
+Qed.
+
+Lemma compile_cu_fname_meta : forall A Ameta B Bmeta fname m,
+    compile_cu (A, Ameta) = Some (B, Bmeta) ->
+    nth_error Bmeta fname = Some m ->
+    m_access m = Public ->
+    nth_error Ameta fname = Some m.
+intros0 Hcomp Hnth Hpub.
+
+fwd eapply compile_cu_meta_split as HH; eauto.
+  destruct HH as (Bnew_meta & ? & ?).  subst Bmeta.
+
+destruct (lt_dec fname (length Ameta)); cycle 1.
+  { exfalso. on _, rewrite_fwd nth_error_app2; [ | lia ].
+    fwd i_lem Forall_nth_error. cbv beta in *. congruence. }
+
+on _, rewrite_fwd nth_error_app1; [ | lia ].
+auto.
+Qed.
+
+Lemma compile_cu_fname_meta' : forall A Ameta B Bmeta fname m,
+    compile_cu (A, Ameta) = Some (B, Bmeta) ->
+    nth_error Ameta fname = Some m ->
+    nth_error Bmeta fname = Some m.
+intros0 Hcomp Hnth.
+
+fwd eapply compile_cu_meta_split as HH; eauto.
+  destruct HH as (Bnew_meta & ? & ?).  subst Bmeta.
+
+rewrite nth_error_app1; eauto.
+rewrite <- nth_error_Some. congruence.
+Qed.
+
+Lemma compile_cu_public_value : forall A Ameta B Bmeta v,
+    compile_cu (A, Ameta) = Some (B, Bmeta) ->
+    public_value Bmeta v ->
+    public_value Ameta v.
+induction v using value_ind'; intros0 Hcomp Hpub; invc Hpub.
+- i_ctor. list_magic_on (args, tt).
+- i_ctor.
+  + i_lem compile_cu_fname_meta.
+  + list_magic_on (free, tt).
+Qed.
+
+Lemma compile_cu_public_value' : forall A Ameta B Bmeta v,
+    compile_cu (A, Ameta) = Some (B, Bmeta) ->
+    public_value Ameta v ->
+    public_value Bmeta v.
+induction v using value_ind'; intros0 Hcomp Hpub; invc Hpub.
+- i_ctor. list_magic_on (args, tt).
+- i_ctor.
+  + i_lem compile_cu_fname_meta'.
+  + list_magic_on (free, tt).
+Qed.
+
+Lemma env_ok_nth_error : forall A B NFREES fname abody bbody nfree,
+    env_ok A B NFREES ->
+    nth_error A fname = Some abody ->
+    nth_error B fname = Some bbody ->
+    nth_error NFREES fname = Some nfree ->
+    I_expr B nfree [] abody bbody /\ A.nfree_ok NFREES abody.
+intros0 Henv Ha Hb Hnf.
+invc Henv.
+fwd i_lem Forall3_nth_error.
+  { rewrite firstn_nth_error_lt; eauto.
+    rewrite <- nth_error_Some. congruence. }
+cbv beta in *.
+fwd i_lem Forall_nth_error.
+auto.
+Qed.
+
+
+
+Require Import Semantics.
+
+Section Preservation.
+
+    Variable aprog : A.prog_type.
+    Variable bprog : B.prog_type.
+
+    Hypothesis Hcomp : compile_cu aprog = Some bprog.
+
+    Theorem fsim : Semantics.forward_simulation (A.semantics aprog) (B.semantics bprog).
+    destruct aprog as [A Ameta], bprog as [B Bmeta].
+    fwd eapply compile_cu_env_ok; eauto.
+
+    set (NFREES := map m_nfree Ameta).
+    eapply Semantics.forward_simulation_plus with
+        (match_states := I' A B NFREES)
+        (match_values := @eq value).
+
+    - simpl. intros0 Bcall Hf Ha. invc Bcall. unfold fst, snd in *.
+      fwd eapply compile_cu_public_value with (v := Close fname free); eauto.
+      fwd eapply compile_cu_public_value with (v := av2); eauto.
+      on (public_value Ameta (Close _ _)), invc.
+      fwd i_lem compile_cu_a_length.
+      fwd eapply length_nth_error_Some with (xs := Ameta) (ys := A) as HH; eauto.
+        destruct HH as [abody Habody].
+      fwd i_lem env_ok_nth_error.
+        { erewrite map_nth_error; [ | eauto ]. eauto. }
+        break_and.
+
+      eexists. split.
+      + econstructor.
+        -- eapply IRun with (bextra := []) (nfree := length free).
+           4: reflexivity. 3: reflexivity. 2: i_ctor.
+           simpl. replace (length free) with (m_nfree m). eassumption.
+        -- i_ctor.
+           ++ econstructor. 1: eauto using A.public_value_nfree_ok.
+              list_magic_on (free, tt). i_lem A.public_value_nfree_ok.
+           ++ i_ctor.
+      + i_ctor. i_ctor.
+
+    - simpl. intros0 II Afinal. invc Afinal. invc II. on >I, invc.
+
+      eexists. split. 2: reflexivity.
+      econstructor; eauto.
+      + unfold fst, snd in *. eauto using compile_cu_public_value'.
+
+    - intros0 Astep. intros0 II.
+      eapply splus_semantics_sim, I'_sim; eauto.
+
+    Defined.
+
+    Lemma match_val_eq :
+      Semantics.fsim_match_val _ _ fsim = eq.
+    Proof.
+      unfold fsim. simpl.
+      unfold Semantics.fsim_match_val.
+      break_match. repeat (break_match_hyp; try congruence).
+      try unfold forward_simulation_step in *.
+      try unfold forward_simulation_plus in *.
+      try unfold forward_simulation_star in *.
+      try unfold forward_simulation_star_wf in *.
+      inv Heqf. reflexivity.
+    Qed.
+
+End Preservation.
+*)
